Section 2.2, starting 2.3

TermRewriting/WellFoundedInduction_2_2.lean
@@ -1,8 +1,165 @@
 import TermRewriting.BasicDefinitions_2_1
+import Mathlib.Data.Set.Finite
+import Mathlib.Data.Fintype.Card
 
 variable (R S : α → α → Prop) 
 
-def WFI R := ∀P: α → Prop, (∀x, (∀y, TransClosure R x y → P y) → P x) → ∀x, P x
+@[simp]
+def WFI := ∀P: α → Prop, (∀x, (∀y, TransClosure R x y → P y) → P x) → ∀x, P x
+
+@[simp]
+def wWFI := ∀P: α → Prop, (∀x, (∀y, R x y → P y) → P x) → ∀x, P x
+
+section open Classical
+
+def iter_chain (f : α → α) (x : α) : Nat → α
+  | 0 => x
+  | Nat.succ n => f (iter_chain f x n)
+
+theorem iter_chain_rel : ∀f,(∀x, R x (f x)) → ∀x n, R (iter_chain f x n) (iter_chain f x (Nat.succ n)) := 
+  by intro f h x n
+     conv => rhs; unfold iter_chain
+     apply h
+
+theorem terminating_wWFI : terminating R → wWFI R := 
+  by apply byContradiction
+     simp; intro rterminates P ind y; apply byContradiction; intro start
+     have successor : ∀z: {z : α // ¬P z}, ∃w : {z : α // ¬P z}, R z w := 
+      by intro ⟨z,zprop⟩
+         have ⟨w',wprop'⟩ := not_forall.mp $ zprop ∘ ind z
+         simp at wprop'
+         let w : {z : α // ¬P z} := ⟨w',wprop'.2⟩
+         exists w
+         simp
+         exact wprop'.1
+     have ⟨next,cprop⟩ := skolem.mp successor
+     have root : {z : α // ¬ P z} := ⟨y,start⟩
+     have iter_chain_prop := iter_chain_rel (λ x y => R x.val y.val) next cprop root
+     have trans_dc : isDescendingChain R (λn ↦ (iter_chain next root n).val) := by
+        intro n; simp; apply iter_chain_prop
+     apply rterminates
+     aesop
+
+theorem tcTerminating_WFI : terminating (TransClosure R) → WFI R := 
+  by intro h; exact terminating_wWFI (TransClosure R) h
+
+-- Proof idea. Given the knowledge that if all transitive desendents of
+-- a node have x have P, then x does too, use one-step induction to show
+-- that everything is such that all its transitive descendents have P.
+-- Conclude that everything has P.
+theorem wWFI_WFI : wWFI R → WFI R := 
+  by simp; intro ind P closure
+     let closureProp (x : α) := ∀y, TransClosure R x y → P y
+     have key : ∀x, closureProp x := by
+        apply ind
+        intro x ih z tcstep
+        cases tcstep
+        case a.base step =>
+          apply closure
+          apply ih
+          assumption
+        case a.step w step tcstep =>
+          apply (ih w step)
+          assumption
+     intro x
+     apply closure
+     intro y
+     apply key
 
 /-- Theorem 2.2.1 -/
-theorem terminating_WFI : terminating R → WFI R := by sorry
+theorem terminating_WFI : terminating R → WFI R := by
+  intro h; apply wWFI_WFI; apply terminating_wWFI; assumption
+
+theorem chain_shift : ∀c, isDescendingChain R c → isDescendingChain R (λ n ↦ c (n + 1)) := by
+  intro c chain n; apply chain
+
+theorem chain_lift : ∀c, isDescendingChain R c → isDescendingChain (TransClosure R) c := by
+  intro c chain n; apply TransClosure.base; apply chain
+
+theorem chain_tc_rel : ∀{c}, isDescendingChain R c → ∀{m n}, m < n → TransClosure R (c m) (c n) := by
+  intro c h m n; revert m; induction n <;> intro m lt
+  case zero => contradiction
+  case succ n ih => 
+    cases lt
+    case refl => apply TransClosure.base; apply h
+    case step le =>
+      apply TransClosure.push (y := c n)
+      · apply ih; apply le
+      · apply h
+
+theorem WFI.tc_terminating : WFI R → terminating (TransClosure R) :=
+  by intro wfi; unfold terminating
+     have key : ∀x, ¬∃c, isDescendingChain (TransClosure R) c ∧ c 0 = x := by
+        apply wfi; intro x ih ⟨chain, chainProp, chainEq⟩
+        apply ih (chain 1)
+        · rw [←chainEq]; apply chainProp
+        · exists (λ n ↦ chain (n + 1)); simp; apply chain_shift; assumption
+     intro ⟨chain,absurd⟩
+     apply key; exists chain
+
+/-- Exercise 2.4 -/
+theorem terminating.trans_closure : terminating (TransClosure R) ↔ terminating R := by
+  constructor
+  case mp => intro term ⟨chain, absurd⟩; apply term; exists chain; apply chain_lift; assumption
+  case mpr => intro term; apply WFI.tc_terminating; apply terminating_WFI; assumption
+
+/-- Theorem 2.2.2 -/
+theorem WFI.terminating : WFI R → terminating R := by
+  intro wfi; apply (terminating.trans_closure R).mp; exact WFI.tc_terminating R wfi
+
+@[simp]
+def finitely_branching := ∀x, Set.Finite { z | R x z }
+@[simp]
+def globally_finite := finitely_branching (TransClosure R)
+@[simp]
+def acyclic := ∀x, ¬TransClosure R x x
+
+/-- Lemma 2.2.4 -/
+theorem terminating.finite_local_global : terminating R → finitely_branching R → globally_finite R := by
+  intro term fini; simp
+  apply (terminating_WFI R)
+  · assumption
+  · intro x ih
+    simp_all
+    let f : {y // R x y } → Set α := λy ↦ { z | TransClosure R y.val z }
+    have f_fin : ∀y, Set.Finite (f y) := by
+      intro y; apply ih y; exact TransClosure.base x y.val y.prop
+    let f_union := ⋃ (i : {y // R x y}), f i
+    have : Set.Finite f_union := @Set.finite_iUnion _ _ (fini x) _ f_fin 
+    apply Set.Finite.subset (s := {y | R x y} ∪ f_union)
+    · apply Set.Finite.union <;> aesop
+    · intro z h; cases h
+      case a.ht.base step => exact Or.inl step
+      case a.ht.step w step tcstep =>
+        apply Or.inr; exists (f ⟨w, step⟩); constructor
+        · simp
+        · exact tcstep
+
+theorem acyclic.chain_injection : acyclic R → ∀c, isDescendingChain R c → Function.Injective c := 
+  by intro acyc chain desc x y eq
+     apply byContradiction; intro neq
+     cases Nat.lt_or_gt.mp neq <;> apply acyc (chain x)
+     case h.inl lt => 
+      conv => rhs; rw [eq]
+      apply chain_tc_rel <;> aesop
+     case h.inr lt =>
+      conv => lhs; rw [eq]
+      apply chain_tc_rel <;> aesop
+
+theorem acyclic.tc_infinite : acyclic R → ∀{c}, isDescendingChain R c → Infinite { z // TransClosure R (c 0) z } :=
+  by intro acyc chain desc
+     let f : Nat → { z // TransClosure R (chain 0) z } := 
+        λn ↦ ⟨chain (n + 1), chain_tc_rel R desc (Nat.zero_lt_succ n)⟩
+     apply Infinite.of_injective f
+     intro x y eq
+     have eq_c : (f x).val = (f y).val := by rw [eq]
+     have := acyclic.chain_injection R acyc chain desc eq_c
+     simp_all
+
+/-- Lemma 2.2.5 -/
+theorem acyclic.globally_finite_terminates : 
+  acyclic R → globally_finite R → terminating R := by
+  intro acyc fini ⟨chain,desc⟩
+  have infini : Infinite { z // TransClosure R (chain 0) z } := acyclic.tc_infinite R acyc desc
+  apply infini.not_finite
+  apply fini
