TermRewriting/ProvingTermination_2_3.lean
@@ -1,0 +1,38 @@
+import TermRewriting.WellFoundedInduction_2_2
+
+variable (R : α → α → Prop) 
+variable (S : β → β → Prop) 
+
+def monotoneIn (R : α → α → Prop) (S : β → β → Prop) (f : α → β) := ∀{x y}, R x y → S (f x) (f y)
+
+theorem monotoneIn.termination : ∀{f}, monotoneIn R S f → terminating S → terminating R := by
+  intro f mono term ⟨chain, desc⟩
+  apply term
+  exists (f ∘ chain)
+  intro n
+  apply mono
+  apply desc
+
+theorem Nat.lt_terminating : terminating (λ x y => ¬Nat.le x y) := by
+  have : ∀n k, k ≤ n → ¬∃c, c 0 = k ∧ isDescendingChain (λ x y => ¬Nat.le x y) c := by
+    intro n; induction n
+    case zero => intro k le ⟨chain, eq, desc⟩; have := desc 0; simp_all
+    case succ n ih => 
+      intro k lt ⟨chain, eq, desc⟩
+      apply ih (chain 1)
+      · have := desc 0; simp_all; omega
+      · exists λn ↦ chain (n + 1); constructor
+        · rfl
+        · simp_all; apply chain_shift (λ x y => y < x) chain desc
+  intro ⟨chain, desc⟩
+  apply this (chain 0) (chain 0) <;> try simp
+  exists chain; simp_all
+
+theorem finitely_branching.terminating_iff_monotoneInN : finitely_branching R →
+  (terminating R ↔ ∃f,monotoneIn R (λ x y => ¬Nat.le x y) f) := by
+  intro fin_b; constructor
+  case mpr => intro ⟨f,mono⟩; apply monotoneIn.termination R (λ x y => ¬Nat.le x y) mono; apply Nat.lt_terminating
+  case mp => sorry
+
+
+
