lakefile.lean
@@ -4,6 +4,7 @@ open Lake DSL
 package «TermRewriting»
 
 require aesop from git "https://github.com/JLimperg/aesop"
+require mathlib from git "https://github.com/leanprover-community/mathlib4"
 
 @[default_target]
 lean_lib «TermRewriting»
